reorganized p4light typing files

deps/poulet4/lib/LightTyping/Typing.v
@@ -2,27 +2,10 @@ Require Export Poulet4.LightTyping.ValueTyping
         Poulet4.Monads.Monad Poulet4.Monads.Option.
 Require Poulet4.P4String Poulet4.P4cub.Util.EquivUtil.
 
-Lemma nth_error_some_length : forall {A : Type} n l (a : A),
-    nth_error l n = Some a -> n < length l.
-Proof.
-  intros A n;
-    induction n as [| n IHn];
-    intros [| h l] a Hnth; cbn in *;
-      try discriminate; firstorder lia.
-Qed.
+(** * P4light Typing Definitions *)
 
-(* TODO:
-   Need parametric operations
-   for [PathMap.t] and [Locator]
-   to be shared by
-   the static & dynamic semantics:
-   [lookup : forall {A}, Locator -> path -> PathMap.t A -> option A]
-   [update : forall {A}, Locator -> path -> A -> PathMap.t A -> PathMap.t A]
-   Only the variable-to-value mapping of [state]
-   relates to the type-context analogue. *)
-    
 Section TypingDefs.
-  Context {tags_t : Type} {dummy : Inhabitant tags_t}.
+  Context {tags_t : Type}.
 
   Notation typ := (@P4Type tags_t).
   Notation expr := (@Expression tags_t).
@@ -69,13 +52,14 @@ Section TypingDefs.
              (l : Locator) (τ : typ)
              '({| var_gamma:=vg; const_gamma:=cg |} : gamma_expr)
     : gamma_expr := {| var_gamma:=bind_var_typ l τ vg; const_gamma:=cg |}.
-  
-  Context `{T : @Target tags_t expr}.
 
-  Definition gamma_var_domain (g : gamma_var) (st : state) : Prop :=
+  Definition gamma_var_domain
+             `{T : @Target tags_t expr}
+             (g : gamma_var) (st : state) : Prop :=
     forall l : Locator, typ_of_loc_var l g = None <-> loc_to_sval l st = None.
 
   Definition gamma_var_val_typ
+             `{T : @Target tags_t expr}
              (g : gamma_var) (st : state)
              (gt : genv_typ) : Prop :=
     forall l t v,
@@ -84,17 +68,20 @@ Section TypingDefs.
       exists rt, get_real_type gt t = Some rt /\ val_typ v (normᵗ rt).
 
   Definition gamma_var_prop
+             `{T : @Target tags_t expr}
              (g : gamma_var) (st : state)
              (gt : genv_typ) : Prop :=
     gamma_var_domain g st /\ gamma_var_val_typ g st gt.
   
   Definition gamma_const_domain
+             `{T : @Target tags_t expr}
              (this : path) (g : gamma_const)
              (ge : genv) : Prop :=
     forall l : Locator,
       typ_of_loc_const this l g = None <-> loc_to_sval_const ge this l = None.
 
   Definition gamma_const_val_typ
+             `{T : @Target tags_t expr}
              (this : path) (g : gamma_const)
              (ge : genv) : Prop :=
     forall l t v,
@@ -104,17 +91,19 @@ Section TypingDefs.
             val_typ v (normᵗ rt).
   
   Definition gamma_const_prop
+             `{T : @Target tags_t expr}
              (this : path) (g : gamma_const) (ge : genv) : Prop :=
     gamma_const_domain this g ge /\ gamma_const_val_typ this g ge.
   
   Definition gamma_expr_prop
+             `{T : @Target tags_t expr}
              (this : path) (g : gamma_expr) (st : state) (ge : genv) : Prop :=
     gamma_var_prop g st ge /\ gamma_const_prop this g ge.
   
-  Notation run_expr := (@exec_expr tags_t T).
-  Notation run_stmt := (@exec_stmt tags_t dummy T).
-  Notation run_blk  := (@exec_block tags_t dummy T).
-  Notation run_call := (@exec_call tags_t dummy T).
+  Notation run_expr := (@exec_expr tags_t).
+  Notation run_stmt := (@exec_stmt tags_t).
+  Notation run_blk  := (@exec_block tags_t).
+  Notation run_call := (@exec_call tags_t).
 
   Definition typ_of_expr
              '(MkExpression _ _ t _ : expr) : typ := t.
@@ -132,7 +121,6 @@ Section TypingDefs.
            is_expr_typ t -> is_expr_typ r.
   
   (** Expression typing. *)
-  Unset Printing Notations.
   Definition
     expr_types
     (this : path)     (** Local path. *)
@@ -140,7 +128,8 @@ Section TypingDefs.
     (Γ : gamma_expr)  (** Typing environment. *)
     (e : expr)        (** Expression to type. *)
     : Prop :=
-    forall (read_one_bit : option bool -> bool -> Prop)
+    forall (T : @Target tags_t expr)
+      (read_one_bit : option bool -> bool -> Prop)
       (ge : genv) (st : state),
       delta_genv_prop ge Δ ->            (** The domain of [ge_typ ge] is [Δ]. *)
       read_one_bit_reads read_one_bit -> (** [read_one_bit] is productive. *)
@@ -198,6 +187,7 @@ Section TypingDefs.
     end.
 
   Definition gamma_func_domain
+             `{T : @Target tags_t expr}
              (this : path) (gf : gamma_func)
              (gi : genv_inst) (ge : genv) : Prop := forall (e : expr),
       lookup_func_typ this gf gi e = None <-> lookup_func ge this e = None.
@@ -230,8 +220,8 @@ Section TypingDefs.
         (FExternal class name)
         (MkFunctionType Xs params FunExtern rt).
   
-  (** TODO: stub. *)
   Definition gamma_func_types
+             `{T : @Target tags_t expr}
              (this : path) (d : list string)
              (g : gamma_expr) (gf : gamma_func)
              (gi : genv_inst) (gext : gamma_ext) (ge : genv) : Prop :=
@@ -241,6 +231,7 @@ Section TypingDefs.
       p = p' /\ fundef_funtype_prop d g gext this fd ft.
 
   Definition gamma_func_prop
+             `{T : @Target tags_t expr}
              (this : path) (d : list string)
              (g : gamma_expr) (gf : gamma_func)
              (gi : genv_inst) (gext : gamma_ext) (ge : genv) : Prop :=
@@ -249,6 +240,7 @@ Section TypingDefs.
 
   (** TODO: externs... *)
   Definition gamma_stmt_prop
+             `{T : @Target tags_t expr}
              (this : path) (d : list string)
              (g : gamma_stmt) (ge : genv) (st : state) : Prop :=
     gamma_expr_prop this (expr_gamma g) st ge /\
@@ -272,7 +264,9 @@ Section TypingDefs.
     (Γ Γ' : gamma_stmt) (* Input & output typing environment. *)
     (s : stmt)          (* Statement in question. *)
     : Prop :=
-    forall (read_one_bit : option bool -> bool -> Prop)
+    forall (dummy : Inhabitant tags_t)
+      (T : @Target tags_t expr)
+      (read_one_bit : option bool -> bool -> Prop)
       (ge : genv) (st : state),
       delta_genv_prop ge Δ ->
       read_one_bit_reads read_one_bit ->
@@ -300,7 +294,9 @@ Section TypingDefs.
     (Γ Γ' : gamma_stmt) (* Input & output typing environments. *)
     (blk : block)       (* Statement block. *)
     : Prop :=
-    forall (read_one_bit : option bool -> bool -> Prop)
+    forall (dummy : Inhabitant tags_t)
+      (T : @Target tags_t expr)
+      (read_one_bit : option bool -> bool -> Prop)
       (ge : genv) (st : state),
       delta_genv_prop ge Δ ->
       read_one_bit_reads read_one_bit ->
@@ -317,7 +313,9 @@ Section TypingDefs.
     (Γ : gamma_stmt)  (* Typing environment. *)
     (call : expr)     (* Call expression. *)
     : Prop :=
-    forall (read_one_bit : option bool -> bool -> Prop) (ge : genv) (st : state),
+    forall (dummy : Inhabitant tags_t)
+      (T : @Target tags_t expr)
+      (read_one_bit : option bool -> bool -> Prop) (ge : genv) (st : state),
       delta_genv_prop ge Δ ->
       read_one_bit_reads read_one_bit ->
       gamma_stmt_prop this Δ Γ ge st ->
@@ -339,1033 +337,3 @@ Notation "Δ '~' Γ₁ '⊢ᵦ' blk ⊣ Γ₂ ≀ this"
 Notation "Δ '~' Γ '⊢ᵪ' e ≀ this"
   := (call_types this Δ Γ e)
        (at level 80, no associativity) : type_scope.
-
-(* TODO. *)
-Section Soundness.
-  Context {tags_t : Type}.
-
-  Notation typ := (@P4Type tags_t).
-  Notation expr := (@Expression tags_t).
-  Notation stmt := (@Statement tags_t).
-  Notation block := (@Block tags_t).
-  Notation signal := (@signal tags_t).
-  Notation ident := string.
-  Notation path := (list ident).
-  Notation Sval := (@ValueBase tags_t (option bool)).
-
-  Create HintDb ind_def.
-  
-  Definition
-    ok_get_real_type_ex_def Δ (τ : typ) := forall ge : genv_typ,
-      delta_genv_prop ge Δ ->
-      exists ρ, get_real_type ge τ = Some ρ.
-
-  Local Hint Unfold ok_get_real_type_ex_def : ind_def.
-  
-  Definition
-    ok_get_real_ctrl_ex_def Δ ct := forall ge : @genv_typ tags_t,
-      delta_genv_prop ge Δ ->
-      exists ct', get_real_ctrl ge ct = Some ct'.
-
-  Local Hint Unfold ok_get_real_ctrl_ex_def : ind_def.
-  
-  Definition
-    ok_get_real_func_ex_def Δ ft := forall ge : @genv_typ tags_t,
-      delta_genv_prop ge Δ ->
-      exists ft', get_real_func ge ft = Some ft'.
-
-  Local Hint Unfold ok_get_real_func_ex_def : ind_def.
-
-  Definition
-    ok_get_real_param_ex_def Δ p := forall ge : @genv_typ tags_t,
-      delta_genv_prop ge Δ ->
-      exists p', get_real_param ge p = Some p'.
-
-  Local Hint Unfold ok_get_real_param_ex_def : ind_def.
-  
-  Definition
-    ok_get_real_type_ex_ind :=
-    my_P4Type_ok_ind
-      _ ok_get_real_type_ex_def
-      ok_get_real_ctrl_ex_def
-      ok_get_real_func_ex_def
-      ok_get_real_param_ex_def.
-
-  Lemma delta_genv_prop_remove : forall Δ (ge : @genv_typ tags_t) X,
-      delta_genv_prop ge Δ ->
-      delta_genv_prop (IdentMap.remove X ge) (remove_str X Δ).
-  Proof.
-    intros d ge X H.
-    unfold delta_genv_prop in *.
-    rewrite Forall_forall in *; intros Y HInY.
-    apply in_remove in HInY as [HInYd HYX].
-    unfold IdentMap.get, IdentMap.remove in *.
-    rewrite FuncAsMap.remove_complete by assumption; eauto.
-  Qed.
-
-  Local Hint Resolve delta_genv_prop_remove : core.
-
-  Lemma delta_genv_prop_removes : forall Xs Δ (ge : @genv_typ tags_t),
-      delta_genv_prop ge Δ ->
-      delta_genv_prop (IdentMap.removes Xs ge) (remove_all Δ Xs).
-  Proof.
-    unfold IdentMap.removes, FuncAsMap.removes.
-    intro Xs; induction Xs as [| X Xs IHXs]; intros d ge Hged; cbn; auto.
-  Qed.
-
-  Local Hint Resolve delta_genv_prop_removes : core.
-
-  Lemma list_ok_get_real_type_ex : forall Δ ts,
-      Forall (fun t => Δ ⊢ok t) ts ->
-      Forall
-        (fun τ => forall ge,
-             delta_genv_prop ge Δ ->
-             exists ρ, get_real_type ge τ = Some ρ) ts ->
-      forall ge : @genv_typ tags_t,
-        delta_genv_prop ge Δ ->
-        exists ρs,
-          sequence (map (get_real_type ge) ts) = Some ρs.
-  Proof.
-    intros d ts Hts IHts ge Hge.
-    rewrite Forall_forall in IHts.
-    specialize IHts with (ge := ge).
-    pose proof reduce_inner_impl _ _ _ _ IHts Hge as H; cbn in *.
-    rewrite <- Forall_forall, Forall_exists_factor in H.
-    destruct H as [ts' Hts'].
-    rewrite Forall2_map_l
-      with (R := fun a b => a = Some b) (f := get_real_type ge)
-      in Hts'.
-    rewrite Forall2_sequence_iff in Hts'; eauto.
-  Qed.
-
-  Local Hint Resolve list_ok_get_real_type_ex : core.
-
-  Create HintDb option_monad.
-  Local Hint Unfold option_ret : option_monad.
-  Local Hint Unfold option_bind : option_monad.
-  Local Hint Unfold option_monad : option_monad.
-  Local Hint Unfold option_monad_inst : option_monad.
-  
-  Lemma alist_ok_get_real_type_ex :
-    forall Δ (ts : list (P4String.t tags_t * typ)),
-      Forall (fun t => Δ ⊢ok snd t) ts ->
-      Forall
-        (fun t => forall ge,
-             delta_genv_prop ge Δ ->
-             exists ρ, get_real_type ge (snd t) = Some ρ) ts ->
-      forall ge : @genv_typ tags_t,
-        delta_genv_prop ge Δ -> exists ρs,
-          sequence
-            (map
-               (fun '(a, t) =>
-                  match get_real_type ge t with
-                  | Some t' => Some (a, t')
-                  | None    => None
-                  end) ts) = Some ρs.
-  Proof.
-    intros d xts Hxts IHxts ge Hge.
-    rewrite Forall_forall in IHxts.
-    specialize IHxts with (ge := ge).
-    pose proof reduce_inner_impl _ _ _ _ IHxts Hge as H; cbn in *.
-    rewrite <- Forall_forall, Forall_exists_factor in H.
-    destruct H as [ts' Hts'].
-    rewrite map_pat_both.
-    assert (Hfst : map fst xts = map fst (combine (map fst xts) ts')).
-    { rewrite map_fst_combine; try reflexivity.
-      apply Forall2_length in Hts'.
-      repeat rewrite map_length; assumption. }
-    assert (Hsnd :
-              Forall2
-                (fun a b => get_real_type ge a = Some b)
-                (map snd xts) (map snd (combine (map fst xts) ts'))).
-    { rewrite map_snd_combine.
-      - rewrite <- Forall2_map_l. assumption.
-      - apply Forall2_length in Hts'.
-        repeat rewrite map_length in *; assumption. }
-    rewrite Forall2_map_l
-      with (R := fun a b => a = Some b) (f := fun a => get_real_type ge (snd a))
-      in Hts'.
-    rewrite <- map_map with (f := snd) in Hts'.
-    pose proof conj Hfst Hsnd as H.
-    rewrite <- Forall2_destr_pair_eq in H.
-    rewrite Forall2_map_l
-      with
-        (f :=
-           fun uv =>
-             match get_real_type ge (snd uv) with
-             | Some w => Some (fst uv, w)
-             | None   => None
-             end)
-        (R := fun uv uw => uv = Some uw) in H.
-    rewrite Forall2_sequence_iff in H.
-    autounfold with option_monad in *.
-    rewrite H; eauto.
-  Qed.
-
-  Local Hint Resolve alist_ok_get_real_type_ex : core.
-
-  Lemma list_ok_get_real_param_ex : forall Δ ps,
-      Forall (P4Parameter_ok Δ) ps ->
-      Forall
-        (fun p => forall ge,
-             delta_genv_prop ge Δ -> exists p',
-               get_real_param ge p = Some p')
-        ps -> forall ge : @genv_typ tags_t,
-          delta_genv_prop ge Δ ->
-          exists ps', sequence (map (get_real_param ge) ps) = Some ps'.
-  Proof.
-    intros d ps Hps IHps ge Hged.
-    rewrite Forall_forall in IHps.
-    specialize IHps with (ge := ge).
-    pose proof reduce_inner_impl _ _ _ _ IHps Hged as H; cbn in *.
-    rewrite <- Forall_forall, Forall_exists_factor in H.
-    destruct H as [ps' Hps'].
-    rewrite Forall2_map_l
-      with (R := fun a b => a = Some b) (f := get_real_param ge)
-      in Hps'.
-    rewrite Forall2_sequence_iff in Hps'; eauto.
-  Qed.
-
-  Local Hint Resolve list_ok_get_real_param_ex : core.
-  
-  Lemma ok_get_real_type_ex :
-    forall Δ τ, Δ ⊢ok τ ->
-      ok_get_real_type_ex_def Δ τ.
-  Proof.
-    apply ok_get_real_type_ex_ind;
-      autounfold with ind_def; cbn;
-        autounfold with option_monad; eauto 2.
-    - intros d t n H Hge ge Hdge.
-      apply Hge in Hdge as [r Hr]; rewrite Hr; eauto 2.
-    - intros d ts Hts IHts ge Hge.
-      eapply list_ok_get_real_type_ex in Hts as [ts' Hts']; eauto.
-      autounfold with option_monad in *.
-      rewrite Hts'; eauto.
-    - intros d ts Hts IHts ge Hge.
-      eapply list_ok_get_real_type_ex in Hts as [ts' Hts']; eauto.
-      autounfold with option_monad in *.
-      rewrite Hts'; eauto.
-    - intros d xts Hxts IHxts ge Hge.
-      eapply alist_ok_get_real_type_ex in Hxts as [ts' Hts']; eauto.
-      autounfold with option_monad in *.
-      rewrite Hts'; eauto.
-    - intros d t H Hge ge Hdge.
-      apply Hge in Hdge as [r Hr]; rewrite Hr; eauto 2.
-    - intros d xts Hxts IHxts ge Hge.
-      eapply alist_ok_get_real_type_ex in Hxts as [ts' Hts']; eauto.
-      autounfold with option_monad in *.
-      rewrite Hts'; eauto.
-    - intros d xts Hxts IHxts ge Hge.
-      eapply alist_ok_get_real_type_ex in Hxts as [ts' Hts']; eauto.
-      autounfold with option_monad in *.
-      rewrite Hts'; eauto.
-    - intros d xts Hxts IHxts ge Hge.
-      eapply alist_ok_get_real_type_ex in Hxts as [ts' Hts']; eauto.
-      autounfold with option_monad in *.
-      rewrite Hts'; eauto.
-    - intros d X ot mems H Hot ge Hdge.
-      inversion Hot as [| t Ht]; subst; eauto.
-      specialize Ht with (ge := IdentMap.remove (P4String.str X) ge).
-      assert (HdX :
-                delta_genv_prop
-                  (IdentMap.remove (P4String.str X) ge)
-                  (remove_str (P4String.str X) d)) by eauto.
-      apply Ht in HdX as [rt Hrt]; clear Ht.
-      rewrite Hrt; eauto.
-    - intros d X HXd ge Hge.
-      unfold delta_genv_prop in Hge.
-      rewrite Forall_forall in Hge. eauto.
-    - firstorder.
-    - intros d ct Hct IH ge Hdge.
-      apply IH in Hdge as [ct' Hct'].
-      unfold get_real_ctrl in Hct'.
-      cbn in Hct'; autounfold with option_monad in Hct'.
-      rewrite Hct'; eauto.
-    - intros d ct Hct IH ge Hdge.
-      apply IH in Hdge as [ct' Hct'].
-      unfold get_real_ctrl in Hct'.
-      cbn in Hct'; autounfold with option_monad in Hct'.
-      rewrite Hct'; eauto.
-    - intros d ct Hct IH ge Hdge.
-      apply IH in Hdge as [ft' Hft'].
-      unfold get_real_func in Hft'.
-      cbn in Hft'; autounfold with option_monad in Hft'.
-      rewrite Hft'; eauto.
-    - intros d ds cs Hds IHds Hcs IHcs ge Hged.
-      eapply list_ok_get_real_param_ex in Hds as [ds' Hds']; eauto.
-      eapply list_ok_get_real_param_ex in Hcs as [cs' Hcs']; eauto.
-      unfold get_real_param in Hds'; unfold get_real_param in Hcs'.
-      cbn in Hds', Hcs';
-        autounfold with option_monad in Hcs', Hds'.
-      rewrite Hcs', Hds'; eauto.
-    - intros d Xs Ys ps Hps IHps ge Hged.
-      eapply list_ok_get_real_param_ex in Hps as [ps' Hps']; eauto.
-      + unfold get_real_param in Hps'; cbn in Hps';
-          autounfold with option_monad in Hps'.
-        rewrite Hps'; eauto.
-      + eauto.
-    - intros d t ts Hts IHts Ht IHt ge Hged.
-      eapply list_ok_get_real_type_ex
-        in Hts as [ts' Hts']; eauto.
-      apply IHt in Hged as [t' Ht'].
-      autounfold with option_monad in *.
-      rewrite Ht', Hts'; eauto.
-    - intros d Xs Ys ps t Hps IHps Ht IHt ge Hged.
-      apply delta_genv_prop_removes
-        with (Xs := map P4String.str Xs) in Hged.
-      eapply list_ok_get_real_param_ex
-        in Hps as [ps' Hps']; eauto.
-      apply IHt in Hged as [t' Ht'].
-      rewrite Ht'.
-      unfold get_real_param in Hps';
-        cbn in Hps'; autounfold with option_monad in Hps'.
-      rewrite Hps'; eauto.
-    - intros d Xs ps Hps IHps ge Hged.
-      apply delta_genv_prop_removes
-        with (Xs := map P4String.str Xs) in Hged.
-      eapply list_ok_get_real_param_ex
-        in Hps as [ps' Hps']; eauto.
-      unfold get_real_param in Hps';
-        cbn in Hps'; autounfold with option_monad in Hps'.
-      rewrite Hps'; eauto.
-    - intros d Xs ps k t Hps IHps Ht IHt ge Hged.
-      apply delta_genv_prop_removes
-        with (Xs := map P4String.str Xs) in Hged.
-      eapply list_ok_get_real_param_ex
-        in Hps as [ps' Hps']; eauto.
-      apply IHt in Hged as [t' Ht'].
-      unfold get_real_param in Hps';
-        cbn in Hps'; autounfold with option_monad in Hps'.
-      rewrite Hps'; clear Hps'.
-      unfold get_real_type in Ht';
-        cbn in Ht'; autounfold with option_monad in Ht'.
-      rewrite Ht'; eauto.
-    - intros d b dr t n x Ht IHt ge Hged.
-      apply IHt in Hged as [t' Ht'].
-      unfold get_real_type in Ht';
-        cbn in Ht'; autounfold with option_monad in Ht'.
-      rewrite Ht'; eauto.
-  Qed.
-
-  Local Hint Resolve ok_get_real_type_ex : core.
-  
-  Definition delta_genv_prop_ok_typ_nil_def
-             Δ (t : typ) := forall ge rt,
-      delta_genv_prop ge Δ ->
-      get_real_type ge t = Some rt ->
-      [] ⊢ok rt.
-
-  Local Hint Unfold delta_genv_prop_ok_typ_nil_def : ind_def.
-  
-  Definition delta_genv_prop_ok_ctrl_nil_def
-             Δ (ct : @ControlType tags_t) := forall ge ct',
-      delta_genv_prop ge Δ ->
-      get_real_ctrl ge ct = Some ct' ->
-      ControlType_ok [] ct'.
-
-  Local Hint Unfold delta_genv_prop_ok_ctrl_nil_def : ind_def.
-
-  Definition delta_genv_prop_ok_func_nil_def
-             Δ (ft : @FunctionType tags_t) := forall ge ft',
-      delta_genv_prop ge Δ ->
-      get_real_func ge ft = Some ft' ->
-      FunctionType_ok [] ft'.
-
-  Local Hint Unfold delta_genv_prop_ok_func_nil_def : ind_def.
-
-  Definition delta_genv_prop_ok_param_nil_def
-             Δ (p : @P4Parameter tags_t) := forall ge p',
-      delta_genv_prop ge Δ ->
-      get_real_param ge p = Some p' ->
-      P4Parameter_ok [] p'.
-
-  Local Hint Unfold delta_genv_prop_ok_param_nil_def : ind_def.
-
-  Definition delta_genv_prop_ok_typ_nil_ind :=
-    my_P4Type_ok_ind
-      _ delta_genv_prop_ok_typ_nil_def
-      delta_genv_prop_ok_ctrl_nil_def
-      delta_genv_prop_ok_func_nil_def
-      delta_genv_prop_ok_param_nil_def.
-
-  Ltac some_inv :=
-    match goal with
-    | H: Some _ = Some _ |- _ => inversion H; subst; clear H
-    end.
-
-  Ltac match_some_inv :=
-    match goal with
-    | H: match ?trm with Some _ => _ | None => _ end = Some _
-      |- _ => destruct trm as [? |] eqn:? ; cbn in *;
-            try discriminate
-    end.
-
-  Local Hint Constructors P4Type_ok : core.
-  Local Hint Constructors ControlType_ok : core.
-  Local Hint Constructors FunctionType_ok : core.
-  Local Hint Constructors P4Parameter_ok : core.
-
-  Local Hint Resolve nth_error_some_length : core.
-  Local Hint Resolve nth_error_In : core.
-  Local Hint Resolve nth_error_in_combine : core.
-  Local Hint Resolve ListUtil.nth_error_exists : core.
-  Local Hint Resolve In_nth_error : core.
-    
-  Lemma delta_genv_prop_ok_typ_nil : forall Δ t,
-      Δ ⊢ok t ->
-      delta_genv_prop_ok_typ_nil_def Δ t.
-  Proof.
-    apply delta_genv_prop_ok_typ_nil_ind;
-      autounfold with ind_def; cbn;
-        autounfold with option_monad;
-        try (intros; repeat match_some_inv;
-             some_inv; eauto; assumption).
-    - intros d ts Hts IHts ge r Hge Hr.
-      match_some_inv; some_inv.
-      rewrite Forall_forall in IHts.
-      specialize IHts with (ge := ge).
-      constructor.
-      rewrite Forall_forall.
-      rewrite <- Forall2_sequence_iff, <- Forall2_map_l in Heqo.
-      rewrite Forall2_forall in Heqo.
-      destruct Heqo as [Hlen Htsl].
-      intros x Hxl.
-      apply In_nth_error in Hxl as [n Hn].
-      assert (Htst: exists t, nth_error ts n = Some t).
-      { apply ListUtil.nth_error_exists.
-        rewrite Hlen.
-        eauto using nth_error_some_length. }
-      firstorder eauto.
-    - admit.
-    - admit.
-    - admit.
-    - admit.
-    - admit.
-    - admit.
-    - intros d X HXd ge r Hge Hr.
-      unfold delta_genv_prop in Hge.
-      (* Problem:
-         types bound to names in [genv_typ]
-         may have free type variables... *)
-  Abort.
-  
-  Context {dummy : Inhabitant tags_t} `{T : @Target tags_t expr}.
-
-  Open Scope monad_scope.
-  
-  Notation run_expr := (@exec_expr tags_t dummy T).
-  Notation run_stmt := (@exec_stmt tags_t dummy T).
-  Notation run_blk := (@exec_block tags_t dummy T).
-
-  Local Hint Unfold expr_types : core.
-  Local Hint Constructors exec_expr : core.
-  Local Hint Constructors val_typ : core.
-  Local Hint Constructors exec_val : core.
-  Local Hint Constructors P4Type_ok : core.
-  Local Hint Constructors is_expr_typ : core.
-
-  Variables (this : path) (Δ : list string).
-  
-  Section ExprTyping.
-    Variable (Γ : @gamma_expr tags_t).
-
-    Ltac solve_ex :=
-      match goal with
-      | |- exists rt, Some ?t = Some rt /\ _
-        => exists t; cbn; eauto
-      end.
-    
-    Ltac soundtac :=
-      autounfold with *;
-      intros rob ge st Hdlta Hrob Hg Hok Hise Hgrt;
-      split; eauto;
-      try (intros v Hrn; inversion Hrn; subst; cbn; try solve_ex).
-  
-    Lemma bool_sound : forall tag b dir,
-        Δ ~ Γ ⊢ₑ MkExpression tag (ExpBool b) TypBool dir ≀ this.
-    Proof.
-      intros; soundtac.
-    Qed.
-  
-    Lemma arbitrary_int_sound : forall tag i z dir,
-        Δ ~ Γ ⊢ₑ
-          MkExpression
-          tag (ExpInt (P4Int.Build_t _ i z None)) TypInteger dir ≀ this.
-    Proof.
-      intros; soundtac.
-    Qed.
-    
-    Lemma unsigned_int_sound : forall tag i z w dir,
-        Δ ~ Γ ⊢ₑ
-          MkExpression tag
-          (ExpInt
-             (P4Int.Build_t _ i z (Some (w,false))))
-          (TypBit w) dir ≀ this.
-    Proof.
-      intros tag i z dir; soundtac.
-      (* TODO: need some result about [P4Arith.to_loptbool]. *)
-    Admitted.
-    
-    Lemma signed_int_sound : forall tag i z w dir,
-        Δ ~ Γ ⊢ₑ
-          MkExpression
-          tag
-          (ExpInt (P4Int.Build_t _ i z (Some (w,true))))
-          (TypInt w) dir ≀ this.
-    Proof.
-      intros tag i z dir; soundtac.
-      (* TODO: need some result about [P4Arith.to_loptbool]. *)
-    Admitted.
-    
-    Lemma string_sound : forall tag s dir,
-        Δ ~ Γ ⊢ₑ MkExpression tag (ExpString s) TypString dir ≀ this.
-    Proof.
-      intros; soundtac.
-    Qed.
-    
-    Lemma name_sound : forall tag x loc t dir,
-        is_directional dir = true ->
-        typ_of_loc_var loc Γ = Some t ->
-        Δ ~ Γ ⊢ₑ MkExpression tag (ExpName x loc) t dir ≀ this.
-    Proof.
-      intros i x l t d Hd Hgt; soundtac.
-      - unfold gamma_expr_prop, gamma_var_prop, gamma_var_domain in Hg.
-        destruct Hg as [[Hg _] _].
-        assert (Hv : exists v, loc_to_sval l st = Some v).
-        { destruct (loc_to_sval l st) as [v |] eqn:Hv; eauto.
-          rewrite <- Hg, Hgt in Hv; discriminate. }
-        destruct Hv; eauto.
-      - unfold gamma_expr_prop, gamma_var_prop, gamma_var_val_typ in Hg.
-        destruct Hg as [[_ Hg] _]; eauto.
-      - rewrite Hd in H7; discriminate.
-    Qed.
-
-    Lemma constant_sound : forall tag x loc t dir,
-        is_directional dir = false ->
-        typ_of_loc_const this loc Γ = Some t ->
-        Δ ~ Γ ⊢ₑ MkExpression tag (ExpName x loc) t dir ≀ this.
-    Proof.
-      intros i x l t d Hd Hgt; soundtac.
-      - unfold gamma_expr_prop, gamma_const_prop, gamma_const_domain in Hg.
-        destruct Hg as (_ & Hg & _).
-        assert (Hv : exists v, loc_to_sval_const ge this l = Some v).
-        { destruct (loc_to_sval_const ge this l) as [v |] eqn:Hv; eauto.
-          rewrite <- Hg, Hgt in Hv; discriminate. }
-        destruct Hv; eauto.
-      - rewrite Hd in H7; discriminate.
-      - unfold gamma_expr_prop, gamma_const_prop, gamma_const_val_typ in Hg.
-        destruct Hg as (_ & _ & Hg); eauto.
-    Qed.
-
-    Lemma array_access_sound : forall tag arry idx ts dir n,
-        typ_of_expr arry = TypArray (TypHeader ts) n ->
-        typ_of_expr idx  = TypBit n ->
-        Δ ~ Γ ⊢ₑ arry ≀ this ->
-        Δ ~ Γ ⊢ₑ idx ≀ this ->
-        Δ ~ Γ ⊢ₑ MkExpression
-          tag (ExpArrayAccess arry idx) (TypHeader ts) dir ≀ this.
-    Proof.
-      intros i e1 e2 ts d n Ht1 Ht2 He1 He2;
-        autounfold with * in *.
-      intros rob ge st Hdelta Hrob Hg Hok Hise Hgrt; simpl in *.
-      rewrite Ht1, Ht2 in *.
-      pose proof He1 rob ge st Hdelta Hrob Hg as [[v1 Hev1] He1']; clear He1; auto.
-      pose proof He2 rob ge st Hdelta Hrob Hg as [[v2 Hev2] He2']; clear He2; auto.
-      split.
-      - assert (Hv2': exists v2', sval_to_val rob v2 v2')
-          by eauto using exec_val_exists.
-        pose proof He1' v1 Hev1 as (r1 & Hr1 & Hv1).
-        pose proof He2' v2 Hev2 as (r2 & Hr2 & Hv2).
-        clear He1' He2'. cbn in *; inversion Hr2; subst; clear Hr2; cbn in *.
-        unfold option_bind, option_ret in *.
-        destruct (sequence (map (fun '(x, t) => get_real_type ge t >>| pair x) ts))
-          as [rs |] eqn:Hrs;
-          unfold ">>|",">>=" in *;
-          unfold option_monad_inst, option_monad in *;
-          unfold mret, mbind, option_bind, option_ret in *;
-          unfold option_monad_inst, option_monad in *;
-          rewrite Hrs in Hr1; try discriminate.
-        inversion Hr1; subst; clear Hr1; cbn in *.
-        assert (Hhrs: get_real_type ge (TypHeader ts) = Some (TypHeader rs)).
-        { cbn in *.
-          unfold ">>|",">>=" in *;
-          unfold option_monad_inst, option_monad in *;
-          unfold mret, mbind, option_bind, option_ret in *;
-          unfold option_monad_inst, option_monad in *;
-          rewrite Hrs; reflexivity. }
-        destruct Hv2' as [v2' Hv2'].
-        inversion Hv1; inversion Hv2; inversion Hv2';
-          subst; try discriminate.
-        rename v into bs; inversion H6; subst; clear H6.
-        assert
-          (Hz: exists z, array_access_idx_to_z (ValBaseBit lb') = Some z)
-          by (simpl; eauto); destruct Hz as [z Hz].
-        assert (forall Δ ge (t t' : typ),
-                   delta_genv_prop ge Δ ->
-                   get_real_type ge t = Some t' ->
-                   Δ ⊢ok t -> [] ⊢ok t') by admit.
-        assert (Hrtok : [] ⊢ok (TypHeader rs)) by admit.
-        assert (Huninit : exists v, uninit_sval_of_typ None (TypHeader rs) = Some v)
-          by eauto using is_expr_typ_uninit_sval_of_typ.
-        destruct Huninit as [v Hv]; eauto.
-      - clear v1 v2 Hev1 Hev2.
-        intros v Hev; inversion Hev; subst.
-        apply He1' in H10 as (r1 & Hr1 & Hv1); clear He1'.
-        apply He2' in H4 as (r2 & Hr2 & Hv2); clear He2'.
-        rewrite H11.
-        unfold get_real_type in Hr1, H11;
-          fold (@get_real_type tags_t) in Hr1, H11.
-        rewrite H11 in Hr1.
-        cbv in Hr1; inversion Hr1; subst; clear Hr1 H11.
-        cbn in *; inversion Hr2; subst; clear Hr2.
-        inversion Hv1; subst.
-        eexists; split; eauto; cbn in *.
-        unfold Znth_def.
-        destruct (ZArith_dec.Z_lt_dec idxz Z0) as [Hidxz | Hidxz].
-        + pose proof uninit_sval_of_typ_val_typ rtyp as H.
-          eapply H; eauto.
-          assert (Hisv: forall A (v : @ValueBase A) (t : typ), val_typ v t -> is_expr_typ t) by admit.
-          apply Hisv in Hv1 as Hv1'.
-          inversion Hv1'; subst.
-          rewrite H1 in H3.
-          assert (Hisn: forall t : typ, is_expr_typ (normᵗ t) -> is_expr_typ t) by admit.
-          auto.
-        + rewrite <- nth_default_eq.
-          unfold nth_default.
-          destruct (nth_error headers (BinInt.Z.to_nat idxz)) as [v |] eqn:Hv.
-          * inversion Hv1; subst.
-            rewrite Forall_forall in H1.
-            eauto using nth_error_In.
-          * pose proof uninit_sval_of_typ_val_typ rtyp as H.
-            eapply H; eauto.
-            assert (Hisv: forall A (v : @ValueBase A) (t : typ), val_typ v t -> is_expr_typ t) by admit.
-            apply Hisv in Hv1 as Hv1'.
-            inversion Hv1'; subst.
-            rewrite H1 in H3.
-            assert (Hisn: forall t : typ, is_expr_typ (normᵗ t) -> is_expr_typ t) by admit.
-            auto.
-    Admitted.
-
-    Lemma bigstring_access_sound : forall tag bits lo hi dir w,
-        (lo <= hi < w)%N ->
-        typ_of_expr bits = TypBit w ->
-        Δ ~ Γ ⊢ₑ bits ≀ this ->
-        Δ ~ Γ ⊢ₑ MkExpression
-          tag (ExpBitStringAccess bits lo hi)
-          (TypBit (hi - lo + 1)%N) dir ≀ this.
-    Proof.
-      intros i e lo hi d w Hlwh Ht He.
-      autounfold with * in *.
-      intros rob ge st Hrob Hg Hok.
-      rewrite Ht in *.
-      pose proof He rob ge st Hrob Hg as [[v Hev] He']; clear He; auto.
-      (*split.
-      - apply He' in Hev as Hv;
-          inversion Hv; subst; rename v0 into bits.
-        exists (ValBaseBit (bitstring_slice bits (N.to_nat lo) (N.to_nat hi))).
-        eapply exec_expr_bitstring_access with (wn := length bits); eauto; lia.
-      - clear v Hev. intros v Hrn; inversion Hrn; subst; simpl.
-        (*rename H8 into He; rename H9 into Hsval; rename H12 into Hlhw.*)
-        (* Need result about [bitstring_slice]. *) admit. *)
-    Admitted.
-  
-    Lemma list_sound : forall tag es dir,
-        Forall (fun e => Δ ~ Γ ⊢ₑ e ≀ this) es ->
-        Δ ~ Γ ⊢ₑ MkExpression tag (ExpList es)
-          (TypTuple (map typ_of_expr es)) dir ≀ this.
-    Proof.
-      intros i es d Hes. autounfold with * in *.
-      intros rob ge st Hrob Hg Hok.
-      rewrite Forall_forall in Hes.
-      specialize Hes with
-          (read_one_bit:=rob) (ge:=ge) (st:=st).
-      pose proof reduce_inner_impl _ _ _ _ Hes Hrob as Hes';
-        simpl in Hes'; clear Hes.
-      pose proof reduce_inner_impl _ _ _ _ Hes' Hg as Hes;
-        simpl in Hes; clear Hes'.
-      simpl in *; inversion Hok;
-        rename H0 into Hτs; rename H into Hτs_eq.
-      rewrite <- Forall_forall in Hes.
-      (*rewrite Forall_map in Hτs.
-      unfold Basics.compose in *.
-      pose proof Forall_impl_Forall _ _ _ _ Hes Hτs as Hq.
-      apply Forall_and_inv in Hq as [Hrnes Htyps]; split.
-      - clear Htyps.
-        rewrite Forall_exists_factor in Hrnes.
-        destruct Hrnes as [vs Hvs]; eauto.
-      - clear Hrnes; intros v Hrn; simpl.
-        inversion Hrn; subst; clear Hrn.
-        rename H6 into Hesvs.
-        rewrite Forall_forall in Htyps.
-        apply forall_Forall2 with (bs := vs) in Htyps;
-          eauto using Forall2_length.
-        apply Forall2_impl with
-            (R := run_expr ge rob this st)
-            (Q := fun e v => val_typ (ge_senum ge) v (typ_of_expr e)) in Htyps; auto.
-        rewrite Forall2_flip, Forall2_map_r in Htyps; auto.
-    Qed.*)
-    Admitted.
-
-    Lemma record_sound : forall tag es dir,
-        Forall (fun e => Δ ~ Γ ⊢ₑ e ≀ this) (map snd es) ->
-        Δ ~ Γ ⊢ₑ MkExpression
-          tag (ExpRecord es)
-          (TypRecord (map (fun '(x,e) => (x,typ_of_expr e)) es)) dir ≀ this.
-    Proof.
-      intros i es d Hes.
-      autounfold with * in *.
-      intros rob ge st Hrob Hg Hok.
-      rewrite Forall_forall in Hes.
-      specialize Hes with
-          (read_one_bit:=rob) (ge:=ge) (st:=st).
-      pose proof reduce_inner_impl _ _ _ _ Hes Hrob as Hes';
-        simpl in Hes'; clear Hes.
-      pose proof reduce_inner_impl _ _ _ _ Hes' Hg as Hes;
-        simpl in Hes; clear Hes'.
-      simpl in *; inversion Hok;
-        rename H0 into Hτs; rename H into Hτs_eq.
-      rewrite <- Forall_forall in Hes.
-      pose proof Forall_map
-           (P4Type_ok Δ) snd
-           (map (fun '(x, e) => (x, typ_of_expr e)) es)
-        as Hfm.
-      unfold Basics.compose in Hfm.
-      (*rewrite <- Hfm in Hτs; clear Hfm.
-      rewrite map_snd_map in Hτs.
-      rewrite Forall_map in Hτs.
-      unfold Basics.compose in *.
-      pose proof Forall_impl_Forall _ _ _ _ Hes Hτs as Hq.
-      apply Forall_and_inv in Hq as [Hrns Htyps]; split.
-      - clear Htyps.
-        rewrite Forall_exists_factor in Hrns.
-        destruct Hrns as [vs Hvs].
-        rewrite AList.Forall2_all_values
-          with (ks := map fst es) in Hvs.
-        + rewrite combine_map_fst_snd in Hvs; eauto. admit.
-        + repeat rewrite map_length; reflexivity.
-        + rewrite map_length, <- map_length with (f := snd).
-          eauto using Forall2_length.
-      - clear Hrns; intros v Hrns.
-        inversion Hrns; subst.
-        rename H6 into Heskvs.
-        rewrite <- combine_map_fst_snd with (l := es)   in Heskvs.
-        rewrite <- combine_map_fst_snd with (l := kvs') in Heskvs.
-        apply AList.all_values_keys_eq in Heskvs as Hmf.
-        repeat rewrite combine_map_fst_snd in Hmf.
-        rewrite <- Hmf in Heskvs.*)
-    (*rewrite <- AList.Forall2_all_values in Heskvs.
-      + constructor; unfold AList.all_values;
-        rewrite Forall2_conj; split.
-        * rewrite Forall2_map_both, Forall2_eq,
-          map_fst_map, map_id; auto.
-        * rewrite Forall2_map_both.
-          rewrite map_snd_map.
-          assert (Hl : length es = length kvs').
-          { rewrite <- map_length with (f := fst) (l := es).
-            rewrite <- map_length with (f := fst) (l := kvs'), Hmf.
-            reflexivity. }
-          rewrite <- map_length with (f := snd) (l := es) in Hl.
-          rewrite <- map_length with (f := snd) (l := kvs') in Hl.
-          pose proof forall_Forall2 _ _ _ _ Htyps (map snd kvs') Hl as Hff2.
-          apply Forall2_impl with
-              (R := run_expr ge rob this st)
-              (Q := fun e v => val_typ (ge_senum ge) v (typ_of_expr e)) in Hff2; auto.
-          rewrite Forall2_flip,Forall2_map_r in Hff2; assumption.
-      + repeat rewrite map_length; reflexivity.
-      + rewrite Hmf; repeat rewrite map_length; reflexivity.
-  Qed.*)
-    Admitted.
-
-    Local Hint Unfold read_detbit : core.
-    Local Hint Unfold sval_to_val : core.
-    Local Hint Unfold val_to_sval : core.
-    
-    Lemma val_to_sval_ex : forall v,
-        val_to_sval v (ValueBaseMap Some v).
-    Proof.
-      autounfold with *; intro v.
-      induction v using (custom_ValueBase_ind bool); simpl; eauto.
-      - constructor.
-        rewrite <- Forall2_map_r, Forall2_Forall, Forall_forall.
-        reflexivity.
-      - constructor.
-        rewrite <- Forall2_map_r, Forall2_Forall, Forall_forall.
-        reflexivity.
-      - constructor.
-        rewrite <- Forall2_map_r, Forall2_Forall, Forall_forall.
-        reflexivity.
-      - constructor.
-        rewrite <- Forall2_map_r, Forall2_Forall.
-        assumption.
-      - constructor. unfold AList.all_values.
-        rewrite <- Forall2_map_r, Forall2_Forall.
-        rewrite Forall_snd in H.
-        apply Forall_and; rewrite Forall_forall in *;
-          intros [? ?]; firstorder.
-      - constructor; auto. unfold AList.all_values.
-        rewrite <- Forall2_map_r, Forall2_Forall.
-        rewrite Forall_snd in H.
-        apply Forall_and; rewrite Forall_forall in *;
-          intros [? ?]; firstorder.
-      - constructor. unfold AList.all_values.
-        rewrite <- Forall2_map_r, Forall2_Forall.
-        rewrite Forall_snd in H.
-        apply Forall_and; rewrite Forall_forall in *;
-          intros [? ?]; firstorder.
-      - constructor.
-        rewrite <- Forall2_map_r, Forall2_Forall.
-        assumption.
-    Qed.
-
-    Local Hint Resolve val_to_sval_ex : core.
-    
-    Lemma eval_unary_op_preserves_typ : forall o v v' t t',
-        unary_type o t t' ->
-        Ops.eval_unary_op o v = Some v' ->
-        val_typ v t -> @val_typ tags_t _ v' t'.
-    Proof.
-      intros o v v' t t' Hut Heval Hvt;
-        inversion Hut; subst;
-          inversion Hvt; subst;
-            try (inversion Heval; subst; auto; assumption).
-      - unfold Ops.eval_unary_op in Heval.
-        destruct (P4Arith.BitArith.from_lbool v0)
-          as [w' n'] eqn:Heqfromlbool.
-        injection Heval as Hv'. rewrite <- Hv'.
-        inversion H; subst; clear H.
-    (** TODO: need helper lemma about
-        [P4Arith.to_lbool] and [P4Arith.BitArith.bit_not]. *)
-    Admitted.
-  
-    Lemma unary_op_sound : forall tag o e t dir,
-        unary_type o (typ_of_expr e) t ->
-        Δ ~ Γ ⊢ₑ e ≀ this ->
-        Δ ~ Γ ⊢ₑ MkExpression tag (ExpUnaryOp o e) t dir ≀ this.
-    Proof.
-      intros i o e t d Hut He.
-      autounfold with * in *; intros rob ge st Hrob Hg Hok.
-      specialize He with rob ge st.
-      simpl in *.
-      apply unary_type_eq in Hut as Hut_eq.
-      rewrite Hut_eq in He.
-      (*pose proof He Hrob Hg Hok as [[v Hev] Hvt]; clear He; split.
-      - apply Hvt in Hev as Hv; clear Hvt.
-        assert (exists v', sval_to_val rob v v')
-          by eauto using exec_val_exists.
-        destruct H as [v' Hv'].
-        assert (exists v''', Ops.eval_unary_op o v' = Some v''').
-        (* Maybe try to factor this out?
-           Lemma exists_eval_unary_op : forall o v,
-           exists v', Ops.eval_unary_op o v = Some v'. *)
-        { destruct (Ops.eval_unary_op o v') as [v'' |] eqn:Heqop; eauto.
-          inversion Hut; subst; try inv_numeric; try inv_numeric_width;
-            match goal with
-            | H: _ = typ_of_expr ?e,
-                 Hv: val_typ _ ?v (typ_of_expr ?e),
-                     Hv': sval_to_val _ ?v _
-              |- _ => rewrite <- H in *; inversion Hv; inversion Hv'; subst
-            end; simpl in *; try discriminate. }
-        firstorder eauto. admit.
-      - clear v Hev; intros v Hev.
-        inversion Hev; subst; simpl in *.
-        pose proof Hvt _ H7 as Hargsv.
-        pose proof
-             (@exec_val_preserves_typ
-                tags_t _ _ _ _ _ H8 (ge_senum ge)) as Hevpt.
-        assert (Hgsb : exists gsb,
-                   FuncAsMap.related
-                     (AList.all_values (exec_val rob))
-                     (ge_senum ge) gsb).
-        { admit. }
-        destruct Hgsb as [gsb Hgsb].
-        pose proof Hevpt _ Hgsb _ Hargsv as Hargv.
-        assert (Hv0: val_typ gsb v0 (typ_of_expr e))
-          by eauto using eval_unary_op_preserves_typ.
-        assert (Hgsb' :
-                  FuncAsMap.related
-                    (AList.all_values val_to_sval)
-                    gsb (ge_senum ge)).
-        { (* TODO:
-             Need assumption
-             [read_one_bit_inverse rob read_detbit]. *)
-          admit. }
-        eauto using exec_val_preserves_typ.*)
-    Admitted.
-
-    Lemma binary_op_sound : forall tag o t e1 e2 dir,
-        binary_type o (typ_of_expr e1) (typ_of_expr e2) t ->
-        Δ ~ Γ ⊢ₑ e1 ≀ this ->
-        Δ ~ Γ ⊢ₑ e2 ≀ this ->
-        Δ ~ Γ ⊢ₑ MkExpression tag (ExpBinaryOp o (e1,e2)) t dir ≀ this.
-    Proof.
-    Admitted.
-  
-    Lemma cast_sound : forall tag e t dir,
-        cast_type (typ_of_expr e) t ->
-        Δ ~ Γ ⊢ₑ e ≀ this ->
-        Δ ~ Γ ⊢ₑ MkExpression tag (ExpCast t e) t dir ≀ this.
-    Proof.
-    Admitted.
-
-    Lemma enum_member_sound : forall tag tname member ename members dir,
-        (* TODO: need [ge] of [genv].
-           name_to_type ge tname = Some (TypEnum ename None members) ->*)
-        List.In member members ->
-        Δ ~ Γ ⊢ₑ MkExpression
-          tag (ExpTypeMember tname member)
-          (TypEnum ename None members) dir ≀ this.
-    Proof.
-    Admitted.
-
-    Lemma senum_member_sound : forall tag tname member ename t members dir,
-        (*name_to_type ge tname = Some (TypEnum ename (Some etyp) members) ->
-          IdentMap.get ename (ge_senum ge) = Some fields ->*)
-        List.In member members ->
-        Δ ~ Γ ⊢ₑ MkExpression
-          tag (ExpTypeMember tname member)
-          (TypEnum ename (Some t) members) dir ≀ this.
-    Proof.
-    Admitted.
-
-    Lemma error_member_sound : forall tag err dir,
-        Δ ~ Γ ⊢ₑ MkExpression
-          tag (ExpErrorMember err) TypError dir ≀ this.
-    Proof.
-      soundtac.
-    Qed.
-  
-    Lemma other_member_sound : forall tag e x ts t dir,
-      member_type ts (typ_of_expr e) ->
-      AList.get ts x = Some t ->
-      Δ ~ Γ ⊢ₑ e ≀ this ->
-      Δ ~ Γ ⊢ₑ MkExpression
-        tag (ExpExpressionMember e x) t dir ≀ this.
-    Proof.
-    Admitted.
-
-    Lemma array_size_sound : forall tag e x dir t w,
-        (* P4Arith.BitArith.bound 32 w -> *)
-        (w < 2 ^ 32)%N ->
-        typ_of_expr e = TypArray t w ->
-        P4String.str x = "size"%string ->
-        Δ ~ Γ ⊢ₑ e ≀ this ->
-        Δ ~ Γ ⊢ₑ MkExpression
-          tag (ExpExpressionMember e x) (TypBit 32) dir ≀ this.
-    Proof.
-    Admitted.
-
-    Lemma array_last_index_sound : forall tag e x dir t w,
-        typ_of_expr e = TypArray t w ->
-        P4String.str x = "lastIndex"%string ->
-        Δ ~ Γ ⊢ₑ e ≀ this ->
-        Δ ~ Γ ⊢ₑ MkExpression
-          tag (ExpExpressionMember e x) t dir ≀ this.
-    Proof.
-    Admitted.
-
-    Lemma ternary_sound : forall tag e₁ e₂ e₃ t dir,
-        typ_of_expr e₁ = TypBool ->
-        typ_of_expr e₂ = typ_of_expr e₃ ->
-        typ_of_expr e₂ = t ->
-        Δ ~ Γ ⊢ₑ e₁ ≀ this ->
-        Δ ~ Γ ⊢ₑ e₂ ≀ this ->
-        Δ ~ Γ ⊢ₑ e₃ ≀ this ->
-        Δ ~ Γ ⊢ₑ MkExpression tag (ExpTernary e₁ e₂ e₃) t dir ≀ this.
-    Proof.
-    Admitted.
-
-    Lemma dontcare_sound : forall tag dir,
-        Δ ~ Γ ⊢ₑ MkExpression tag ExpDontCare TypVoid dir ≀ this.
-    Proof.
-      soundtac.
-    Qed.
-  End ExprTyping.
-
-  Local Hint Constructors exec_stmt : core.
-  Local Hint Constructors exec_block : core.
-  
-  Section StmtTyping.
-    Variable (Γ : @gamma_stmt tags_t).
-    
-    Lemma assign_sound : forall tag e₁ e₂,
-        typ_of_expr e₁ = typ_of_expr e₂ ->
-        lexpr_ok e₁ ->
-        Δ ~ Γ ⊢ₑ e₁ ≀ this ->
-        Δ ~ Γ ⊢ₑ e₂ ≀ this \/ Δ ~ Γ ⊢ᵪ e₂ ≀ this ->
-        Δ ~ Γ ⊢ₛ MkStatement
-          tag (StatAssignment e₁ e₂) StmUnit ⊣ Γ ≀ this.
-    Proof.
-    Admitted.
-
-    Lemma cond_sound : forall tag e s₁ s₂ Γ₁,
-        typ_of_expr e = TypBool ->
-        Δ ~ Γ ⊢ₑ e ≀ this ->
-        Δ ~ Γ ⊢ₛ s₁ ⊣ Γ₁ ≀ this ->
-        predopt (fun s₂ => exists Γ₂, Δ ~ Γ ⊢ₛ s₂ ⊣ Γ₂ ≀ this) s₂ ->
-        Δ ~ Γ ⊢ₛ MkStatement
-          tag (StatConditional e s₁ s₂)
-          (match s₂ with
-           | None    => typ_of_stmt s₁
-           | Some s₂ => lub_StmType (typ_of_stmt s₁) (typ_of_stmt s₂)
-           end) ⊣ Γ ≀ this.
-    Proof.
-    Admitted.
-
-    Lemma exit_sound : forall tag,
-        Δ ~ Γ ⊢ₛ MkStatement tag StatExit StmVoid ⊣ Γ ≀ this.
-    Proof.
-      unfold stmt_types; intros; split; eauto.
-      intros ? ? Hrn; inversion Hrn; subst; eauto.
-    Qed.
-
-    Lemma return_sound : forall tag e,
-        predopt (fun e => Δ ~ Γ ⊢ₑ e ≀ this) e ->
-        Δ ~ Γ ⊢ₛ MkStatement tag (StatReturn e) StmVoid ⊣ Γ ≀ this.
-    Proof.
-    Admitted.
-
-    Lemma empty_sound : forall tag,
-        Δ ~ Γ ⊢ₛ MkStatement tag StatEmpty StmUnit ⊣ Γ ≀ this.
-    Proof.
-      unfold stmt_types; intros; split; eauto.
-      intros ? ? Hrn; inversion Hrn; subst; eauto.
-    Qed.
-    
-    Lemma block_sound : forall Γ' tag blk t,
-        Block_StmTypes blk t ->
-        Δ ~ Γ ⊢ᵦ blk ⊣ Γ' ≀ this ->
-        Δ ~ Γ ⊢ₛ MkStatement tag (StatBlock blk) t ⊣ Γ ≀ this.
-    Proof.
-    Admitted.
-
-    Lemma method_call_sound : forall tag e τs es,
-        Δ ~ Γ ⊢ᵪ MkExpression dummy_tags
-          (ExpFunctionCall e τs es)
-          TypVoid Directionless ≀ this ->
-        Δ ~ Γ ⊢ₛ MkStatement tag
-          (StatMethodCall e τs es) StmUnit ⊣ Γ ≀ this.
-    Proof.
-    Admitted.
-
-    Lemma direct_application_sound : forall tag τ es,
-        Δ ~ Γ ⊢ₑ MkExpression dummy_tags
-          (ExpFunctionCall
-             (direct_application_expression τ)
-             nil (map Some es)) TypVoid Directionless ≀ this ->
-        Δ ~ Γ ⊢ₛ MkStatement tag
-          (StatDirectApplication τ es) StmUnit ⊣ Γ ≀ this.
-    Proof.
-    Admitted.
-
-    Lemma stat_variable_sound : forall tag τ x e l,
-        predopt
-          (fun e =>
-             typ_of_expr e = τ /\
-             (Δ ~ Γ ⊢ₑ e ≀ this \/ Δ ~ Γ ⊢ᵪ e ≀ this)) e ->
-        Δ ~ Γ ⊢ₛ MkStatement
-          tag (StatVariable τ x e l) StmUnit
-          ⊣ bind_typ_gamma_stmt l τ Γ ≀ this.
-    Proof.
-    Admitted.
-  End StmtTyping.
-End Soundness.
