deps/poulet4/lib/LightTyping/Lemmas.v
@@ -1,0 +1,403 @@
+Require Export Poulet4.LightTyping.Typing.
+
+Section Lemmas.
+  Context {tags_t : Type}.
+
+  Notation typ := (@P4Type tags_t).
+  Notation ident := string.
+  Notation path := (list ident).
+
+  Create HintDb ind_def.
+  
+  Definition
+    ok_get_real_type_ex_def Δ (τ : typ) := forall ge : genv_typ,
+      delta_genv_prop ge Δ ->
+      exists ρ, get_real_type ge τ = Some ρ.
+
+  Local Hint Unfold ok_get_real_type_ex_def : ind_def.
+  
+  Definition
+    ok_get_real_ctrl_ex_def Δ ct := forall ge : @genv_typ tags_t,
+      delta_genv_prop ge Δ ->
+      exists ct', get_real_ctrl ge ct = Some ct'.
+
+  Local Hint Unfold ok_get_real_ctrl_ex_def : ind_def.
+  
+  Definition
+    ok_get_real_func_ex_def Δ ft := forall ge : @genv_typ tags_t,
+      delta_genv_prop ge Δ ->
+      exists ft', get_real_func ge ft = Some ft'.
+
+  Local Hint Unfold ok_get_real_func_ex_def : ind_def.
+
+  Definition
+    ok_get_real_param_ex_def Δ p := forall ge : @genv_typ tags_t,
+      delta_genv_prop ge Δ ->
+      exists p', get_real_param ge p = Some p'.
+
+  Local Hint Unfold ok_get_real_param_ex_def : ind_def.
+  
+  Definition
+    ok_get_real_type_ex_ind :=
+    my_P4Type_ok_ind
+      _ ok_get_real_type_ex_def
+      ok_get_real_ctrl_ex_def
+      ok_get_real_func_ex_def
+      ok_get_real_param_ex_def.
+
+  Lemma delta_genv_prop_remove : forall Δ (ge : @genv_typ tags_t) X,
+      delta_genv_prop ge Δ ->
+      delta_genv_prop (IdentMap.remove X ge) (remove_str X Δ).
+  Proof.
+    intros d ge X H.
+    unfold delta_genv_prop in *.
+    rewrite Forall_forall in *; intros Y HInY.
+    apply in_remove in HInY as [HInYd HYX].
+    unfold IdentMap.get, IdentMap.remove in *.
+    rewrite FuncAsMap.remove_complete by assumption; eauto.
+  Qed.
+
+  Local Hint Resolve delta_genv_prop_remove : core.
+
+  Lemma delta_genv_prop_removes : forall Xs Δ (ge : @genv_typ tags_t),
+      delta_genv_prop ge Δ ->
+      delta_genv_prop (IdentMap.removes Xs ge) (remove_all Δ Xs).
+  Proof.
+    unfold IdentMap.removes, FuncAsMap.removes.
+    intro Xs; induction Xs as [| X Xs IHXs]; intros d ge Hged; cbn; auto.
+  Qed.
+
+  Local Hint Resolve delta_genv_prop_removes : core.
+
+  Lemma list_ok_get_real_type_ex : forall Δ ts,
+      Forall (fun t => Δ ⊢ok t) ts ->
+      Forall
+        (fun τ => forall ge,
+             delta_genv_prop ge Δ ->
+             exists ρ, get_real_type ge τ = Some ρ) ts ->
+      forall ge : @genv_typ tags_t,
+        delta_genv_prop ge Δ ->
+        exists ρs,
+          sequence (map (get_real_type ge) ts) = Some ρs.
+  Proof.
+    intros d ts Hts IHts ge Hge.
+    rewrite Forall_forall in IHts.
+    specialize IHts with (ge := ge).
+    pose proof reduce_inner_impl _ _ _ _ IHts Hge as H; cbn in *.
+    rewrite <- Forall_forall, Forall_exists_factor in H.
+    destruct H as [ts' Hts'].
+    rewrite Forall2_map_l
+      with (R := fun a b => a = Some b) (f := get_real_type ge)
+      in Hts'.
+    rewrite Forall2_sequence_iff in Hts'; eauto.
+  Qed.
+
+  Local Hint Resolve list_ok_get_real_type_ex : core.
+
+  Create HintDb option_monad.
+  Local Hint Unfold option_ret : option_monad.
+  Local Hint Unfold option_bind : option_monad.
+  Local Hint Unfold option_monad : option_monad.
+  Local Hint Unfold option_monad_inst : option_monad.
+  
+  Lemma alist_ok_get_real_type_ex :
+    forall Δ (ts : list (P4String.t tags_t * typ)),
+      Forall (fun t => Δ ⊢ok snd t) ts ->
+      Forall
+        (fun t => forall ge,
+             delta_genv_prop ge Δ ->
+             exists ρ, get_real_type ge (snd t) = Some ρ) ts ->
+      forall ge : @genv_typ tags_t,
+        delta_genv_prop ge Δ -> exists ρs,
+          sequence
+            (map
+               (fun '(a, t) =>
+                  match get_real_type ge t with
+                  | Some t' => Some (a, t')
+                  | None    => None
+                  end) ts) = Some ρs.
+  Proof.
+    intros d xts Hxts IHxts ge Hge.
+    rewrite Forall_forall in IHxts.
+    specialize IHxts with (ge := ge).
+    pose proof reduce_inner_impl _ _ _ _ IHxts Hge as H; cbn in *.
+    rewrite <- Forall_forall, Forall_exists_factor in H.
+    destruct H as [ts' Hts'].
+    rewrite map_pat_both.
+    assert (Hfst : map fst xts = map fst (combine (map fst xts) ts')).
+    { rewrite map_fst_combine; try reflexivity.
+      apply Forall2_length in Hts'.
+      repeat rewrite map_length; assumption. }
+    assert (Hsnd :
+              Forall2
+                (fun a b => get_real_type ge a = Some b)
+                (map snd xts) (map snd (combine (map fst xts) ts'))).
+    { rewrite map_snd_combine.
+      - rewrite <- Forall2_map_l. assumption.
+      - apply Forall2_length in Hts'.
+        repeat rewrite map_length in *; assumption. }
+    rewrite Forall2_map_l
+      with (R := fun a b => a = Some b) (f := fun a => get_real_type ge (snd a))
+      in Hts'.
+    rewrite <- map_map with (f := snd) in Hts'.
+    pose proof conj Hfst Hsnd as H.
+    rewrite <- Forall2_destr_pair_eq in H.
+    rewrite Forall2_map_l
+      with
+        (f :=
+           fun uv =>
+             match get_real_type ge (snd uv) with
+             | Some w => Some (fst uv, w)
+             | None   => None
+             end)
+        (R := fun uv uw => uv = Some uw) in H.
+    rewrite Forall2_sequence_iff in H.
+    autounfold with option_monad in *.
+    rewrite H; eauto.
+  Qed.
+
+  Local Hint Resolve alist_ok_get_real_type_ex : core.
+
+  Lemma list_ok_get_real_param_ex : forall Δ ps,
+      Forall (P4Parameter_ok Δ) ps ->
+      Forall
+        (fun p => forall ge,
+             delta_genv_prop ge Δ -> exists p',
+               get_real_param ge p = Some p')
+        ps -> forall ge : @genv_typ tags_t,
+          delta_genv_prop ge Δ ->
+          exists ps', sequence (map (get_real_param ge) ps) = Some ps'.
+  Proof.
+    intros d ps Hps IHps ge Hged.
+    rewrite Forall_forall in IHps.
+    specialize IHps with (ge := ge).
+    pose proof reduce_inner_impl _ _ _ _ IHps Hged as H; cbn in *.
+    rewrite <- Forall_forall, Forall_exists_factor in H.
+    destruct H as [ps' Hps'].
+    rewrite Forall2_map_l
+      with (R := fun a b => a = Some b) (f := get_real_param ge)
+      in Hps'.
+    rewrite Forall2_sequence_iff in Hps'; eauto.
+  Qed.
+
+  Local Hint Resolve list_ok_get_real_param_ex : core.
+  
+  Lemma ok_get_real_type_ex :
+    forall Δ τ, Δ ⊢ok τ ->
+      ok_get_real_type_ex_def Δ τ.
+  Proof.
+    apply ok_get_real_type_ex_ind;
+      autounfold with ind_def; cbn;
+        autounfold with option_monad; eauto 2.
+    - intros d t n H Hge ge Hdge.
+      apply Hge in Hdge as [r Hr]; rewrite Hr; eauto 2.
+    - intros d ts Hts IHts ge Hge.
+      eapply list_ok_get_real_type_ex in Hts as [ts' Hts']; eauto.
+      autounfold with option_monad in *.
+      rewrite Hts'; eauto.
+    - intros d ts Hts IHts ge Hge.
+      eapply list_ok_get_real_type_ex in Hts as [ts' Hts']; eauto.
+      autounfold with option_monad in *.
+      rewrite Hts'; eauto.
+    - intros d xts Hxts IHxts ge Hge.
+      eapply alist_ok_get_real_type_ex in Hxts as [ts' Hts']; eauto.
+      autounfold with option_monad in *.
+      rewrite Hts'; eauto.
+    - intros d t H Hge ge Hdge.
+      apply Hge in Hdge as [r Hr]; rewrite Hr; eauto 2.
+    - intros d xts Hxts IHxts ge Hge.
+      eapply alist_ok_get_real_type_ex in Hxts as [ts' Hts']; eauto.
+      autounfold with option_monad in *.
+      rewrite Hts'; eauto.
+    - intros d xts Hxts IHxts ge Hge.
+      eapply alist_ok_get_real_type_ex in Hxts as [ts' Hts']; eauto.
+      autounfold with option_monad in *.
+      rewrite Hts'; eauto.
+    - intros d xts Hxts IHxts ge Hge.
+      eapply alist_ok_get_real_type_ex in Hxts as [ts' Hts']; eauto.
+      autounfold with option_monad in *.
+      rewrite Hts'; eauto.
+    - intros d X ot mems H Hot ge Hdge.
+      inversion Hot as [| t Ht]; subst; eauto.
+      specialize Ht with (ge := IdentMap.remove (P4String.str X) ge).
+      assert (HdX :
+                delta_genv_prop
+                  (IdentMap.remove (P4String.str X) ge)
+                  (remove_str (P4String.str X) d)) by eauto.
+      apply Ht in HdX as [rt Hrt]; clear Ht.
+      rewrite Hrt; eauto.
+    - intros d X HXd ge Hge.
+      unfold delta_genv_prop in Hge.
+      rewrite Forall_forall in Hge. eauto.
+    - firstorder.
+    - intros d ct Hct IH ge Hdge.
+      apply IH in Hdge as [ct' Hct'].
+      unfold get_real_ctrl in Hct'.
+      cbn in Hct'; autounfold with option_monad in Hct'.
+      rewrite Hct'; eauto.
+    - intros d ct Hct IH ge Hdge.
+      apply IH in Hdge as [ct' Hct'].
+      unfold get_real_ctrl in Hct'.
+      cbn in Hct'; autounfold with option_monad in Hct'.
+      rewrite Hct'; eauto.
+    - intros d ct Hct IH ge Hdge.
+      apply IH in Hdge as [ft' Hft'].
+      unfold get_real_func in Hft'.
+      cbn in Hft'; autounfold with option_monad in Hft'.
+      rewrite Hft'; eauto.
+    - intros d ds cs Hds IHds Hcs IHcs ge Hged.
+      eapply list_ok_get_real_param_ex in Hds as [ds' Hds']; eauto.
+      eapply list_ok_get_real_param_ex in Hcs as [cs' Hcs']; eauto.
+      unfold get_real_param in Hds'; unfold get_real_param in Hcs'.
+      cbn in Hds', Hcs';
+        autounfold with option_monad in Hcs', Hds'.
+      rewrite Hcs', Hds'; eauto.
+    - intros d Xs Ys ps Hps IHps ge Hged.
+      eapply list_ok_get_real_param_ex in Hps as [ps' Hps']; eauto.
+      + unfold get_real_param in Hps'; cbn in Hps';
+          autounfold with option_monad in Hps'.
+        rewrite Hps'; eauto.
+      + eauto.
+    - intros d t ts Hts IHts Ht IHt ge Hged.
+      eapply list_ok_get_real_type_ex
+        in Hts as [ts' Hts']; eauto.
+      apply IHt in Hged as [t' Ht'].
+      autounfold with option_monad in *.
+      rewrite Ht', Hts'; eauto.
+    - intros d Xs Ys ps t Hps IHps Ht IHt ge Hged.
+      apply delta_genv_prop_removes
+        with (Xs := map P4String.str Xs) in Hged.
+      eapply list_ok_get_real_param_ex
+        in Hps as [ps' Hps']; eauto.
+      apply IHt in Hged as [t' Ht'].
+      rewrite Ht'.
+      unfold get_real_param in Hps';
+        cbn in Hps'; autounfold with option_monad in Hps'.
+      rewrite Hps'; eauto.
+    - intros d Xs ps Hps IHps ge Hged.
+      apply delta_genv_prop_removes
+        with (Xs := map P4String.str Xs) in Hged.
+      eapply list_ok_get_real_param_ex
+        in Hps as [ps' Hps']; eauto.
+      unfold get_real_param in Hps';
+        cbn in Hps'; autounfold with option_monad in Hps'.
+      rewrite Hps'; eauto.
+    - intros d Xs ps k t Hps IHps Ht IHt ge Hged.
+      apply delta_genv_prop_removes
+        with (Xs := map P4String.str Xs) in Hged.
+      eapply list_ok_get_real_param_ex
+        in Hps as [ps' Hps']; eauto.
+      apply IHt in Hged as [t' Ht'].
+      unfold get_real_param in Hps';
+        cbn in Hps'; autounfold with option_monad in Hps'.
+      rewrite Hps'; clear Hps'.
+      unfold get_real_type in Ht';
+        cbn in Ht'; autounfold with option_monad in Ht'.
+      rewrite Ht'; eauto.
+    - intros d b dr t n x Ht IHt ge Hged.
+      apply IHt in Hged as [t' Ht'].
+      unfold get_real_type in Ht';
+        cbn in Ht'; autounfold with option_monad in Ht'.
+      rewrite Ht'; eauto.
+  Qed.
+  
+  Definition delta_genv_prop_ok_typ_nil_def
+             Δ (t : typ) := forall ge rt,
+      delta_genv_prop ge Δ ->
+      get_real_type ge t = Some rt ->
+      [] ⊢ok rt.
+
+  Local Hint Unfold delta_genv_prop_ok_typ_nil_def : ind_def.
+  
+  Definition delta_genv_prop_ok_ctrl_nil_def
+             Δ (ct : @ControlType tags_t) := forall ge ct',
+      delta_genv_prop ge Δ ->
+      get_real_ctrl ge ct = Some ct' ->
+      ControlType_ok [] ct'.
+
+  Local Hint Unfold delta_genv_prop_ok_ctrl_nil_def : ind_def.
+
+  Definition delta_genv_prop_ok_func_nil_def
+             Δ (ft : @FunctionType tags_t) := forall ge ft',
+      delta_genv_prop ge Δ ->
+      get_real_func ge ft = Some ft' ->
+      FunctionType_ok [] ft'.
+
+  Local Hint Unfold delta_genv_prop_ok_func_nil_def : ind_def.
+
+  Definition delta_genv_prop_ok_param_nil_def
+             Δ (p : @P4Parameter tags_t) := forall ge p',
+      delta_genv_prop ge Δ ->
+      get_real_param ge p = Some p' ->
+      P4Parameter_ok [] p'.
+
+  Local Hint Unfold delta_genv_prop_ok_param_nil_def : ind_def.
+
+  Definition delta_genv_prop_ok_typ_nil_ind :=
+    my_P4Type_ok_ind
+      _ delta_genv_prop_ok_typ_nil_def
+      delta_genv_prop_ok_ctrl_nil_def
+      delta_genv_prop_ok_func_nil_def
+      delta_genv_prop_ok_param_nil_def.
+
+  Ltac some_inv :=
+    match goal with
+    | H: Some _ = Some _ |- _ => inversion H; subst; clear H
+    end.
+
+  Ltac match_some_inv :=
+    match goal with
+    | H: match ?trm with Some _ => _ | None => _ end = Some _
+      |- _ => destruct trm as [? |] eqn:? ; cbn in *;
+            try discriminate
+    end.
+
+  Local Hint Constructors P4Type_ok : core.
+  Local Hint Constructors ControlType_ok : core.
+  Local Hint Constructors FunctionType_ok : core.
+  Local Hint Constructors P4Parameter_ok : core.
+
+  Local Hint Resolve nth_error_some_length : core.
+  Local Hint Resolve nth_error_In : core.
+  Local Hint Resolve nth_error_in_combine : core.
+  Local Hint Resolve ListUtil.nth_error_exists : core.
+  Local Hint Resolve In_nth_error : core.
+    
+  Lemma delta_genv_prop_ok_typ_nil : forall Δ t,
+      Δ ⊢ok t ->
+      delta_genv_prop_ok_typ_nil_def Δ t.
+  Proof.
+    apply delta_genv_prop_ok_typ_nil_ind;
+      autounfold with ind_def; cbn;
+        autounfold with option_monad;
+        try (intros; repeat match_some_inv;
+             some_inv; eauto; assumption).
+    - intros d ts Hts IHts ge r Hge Hr.
+      match_some_inv; some_inv.
+      rewrite Forall_forall in IHts.
+      specialize IHts with (ge := ge).
+      constructor.
+      rewrite Forall_forall.
+      rewrite <- Forall2_sequence_iff, <- Forall2_map_l in Heqo.
+      rewrite Forall2_forall in Heqo.
+      destruct Heqo as [Hlen Htsl].
+      intros x Hxl.
+      apply In_nth_error in Hxl as [n Hn].
+      assert (Htst: exists t, nth_error ts n = Some t).
+      { apply ListUtil.nth_error_exists.
+        rewrite Hlen.
+        eauto using nth_error_some_length. }
+      firstorder eauto.
+    - admit.
+    - admit.
+    - admit.
+    - admit.
+    - admit.
+    - admit.
+    - intros d X HXd ge r Hge Hr.
+      unfold delta_genv_prop in Hge.
+      (* Problem:
+         types bound to names in [genv_typ]
+         may have free type variables... *)
+  Abort.
+End Lemmas.
