deps/poulet4/lib/LightTyping/Utility.v
@@ -2,7 +2,8 @@ From Coq Require Export NArith.BinNat Strings.String Lists.List micromega.Lia.
 Require Export Poulet4.Typed Poulet4.Syntax Poulet4.ValueUtil.
 Export ListNotations.
 Require Poulet4.P4String Poulet4.P4cub.Util.EquivUtil.
-Require Import Poulet4.Monads.Monad Poulet4.Monads.Option.
+Require Import Poulet4.Monads.Monad Poulet4.Monads.Option
+        Poulet4.Sublist Poulet4.Utils.
 
 Notation predopt    := (EquivUtil.predop).
 Notation remove_str := (remove string_dec).
@@ -239,6 +240,52 @@ Section Utils.
   | is_newtype X t :
       is_expr_typ t ->
       is_expr_typ (TypNewType X t).
+
+  Fixpoint normᵗ (t : typ) : typ :=
+    match t with
+    | TypBool
+    | TypString
+    | TypInteger
+    | TypInt _
+    | TypBit _
+    | TypVarBit _
+    | TypError
+    | TypMatchKind
+    | TypVoid
+    | TypTypeName _
+    | TypExtern _
+    | TypTable _   => t
+    | TypArray t n => TypArray (normᵗ t) n
+    | TypList  ts
+    | TypTuple ts  => TypTuple (map normᵗ ts)
+    | TypRecord ts
+    | TypStruct ts => TypStruct (map (fun '(x,t) => (x, normᵗ t)) ts)
+    | TypSet    t  => TypSet (normᵗ t)
+    | TypHeader ts => TypHeader (map (fun '(x,t) => (x, normᵗ t)) ts)
+    | TypHeaderUnion ts => TypHeaderUnion (map (fun '(x,t) => (x, normᵗ t)) ts)
+    | TypEnum X t ms    => TypEnum X (option_map normᵗ t) ms
+    | TypNewType _ t    => normᵗ t
+    | TypControl ct             => TypControl (normᶜ ct)
+    | TypParser  ct             => TypParser  (normᶜ ct)
+    | TypFunction ft            => TypFunction (normᶠ ft)
+    | TypAction cs ds           => TypAction (map normᵖ cs) (map normᵖ ds)
+    | TypPackage Xs ws ps       => TypPackage Xs ws (map normᵖ ps)
+    | TypSpecializedType t ts   => TypSpecializedType (normᵗ t) (map normᵗ ts)
+    | TypConstructor Xs ws ps t => TypConstructor Xs ws (map normᵖ ps) (normᵗ t)
+    end
+  with normᶜ (ct : ControlType) : ControlType :=
+         match ct with
+         | MkControlType Xs ps => MkControlType Xs (map normᵖ ps)
+         end
+  with normᶠ (ft : FunctionType) : FunctionType :=
+         match ft with
+         | MkFunctionType Xs ps k t
+           => MkFunctionType Xs (map normᵖ ps) k (normᵗ t)
+         end
+  with normᵖ (p : P4Parameter) : P4Parameter :=
+         match p with
+         | MkParameter b d t a x => MkParameter b d (normᵗ t) a x
+         end.
 End Utils.
 
 Section IsExprTypInd.
@@ -736,10 +783,11 @@ Section OkBoomerInd.
 End OkBoomerInd.
 
 Section Lemmas.
-  Context {tags_t : Type} {dummy : Sublist.Inhabitant tags_t}.
-
+  Context {tags_t : Type}.
+  Notation typ := (@P4Type tags_t).
+  
   Lemma is_expr_typ_list_uninit_sval_of_typ :
-    forall (ts : list (@P4Type tags_t)) b,
+    forall (ts : list (typ)) b,
       Forall is_expr_typ ts ->
       Forall
         (fun t => [] ⊢ok t -> exists v,
@@ -764,7 +812,7 @@ Section Lemmas.
   Local Open Scope monad_scope.
   
   Lemma is_expr_typ_alist_uninit_sval_of_typ :
-    forall (xts : list (P4String.t tags_t * (@P4Type tags_t))) b,
+    forall (xts : list (P4String.t tags_t * (typ))) b,
       Forall (fun xt => is_expr_typ (snd xt)) xts ->
       Forall
         (fun xt =>
@@ -835,7 +883,7 @@ Section Lemmas.
 
   Local Hint Extern 0 => apply_ind : core.
   
-  Lemma is_expr_typ_uninit_sval_of_typ : forall (t : @P4Type tags_t) b,
+  Lemma is_expr_typ_uninit_sval_of_typ : forall (t : typ) b,
     is_expr_typ t -> [] ⊢ok t ->
     exists v, uninit_sval_of_typ b t = Some v.
   Proof.
@@ -895,24 +943,60 @@ Section Lemmas.
           subst; cbn in *; eauto; try lia; eauto.
   Qed.
 
-  Definition uninit_sval_of_typ_is_expr_typ_def (t : @P4Type tags_t) :=
-    forall b v, uninit_sval_of_typ b t = Some v -> is_expr_typ t.
-
-  Definition uninit_sval_of_typ_is_expr_typ_ind :=
+  Definition normᵗ_idem_def (t : typ) := normᵗ (normᵗ t) = normᵗ t.
+  Definition normᶜ_idem_def (t : @ControlType tags_t) := normᶜ (normᶜ t) = normᶜ t.
+  Definition normᶠ_idem_def (t : @FunctionType tags_t) := normᶠ (normᶠ t) = normᶠ t.
+  Definition normᵖ_idem_def (t : @P4Parameter tags_t) := normᵖ (normᵖ t) = normᵖ t.
+  
+  Definition normᵗ_idem_ind :=
     my_P4Type_ind
-      _ uninit_sval_of_typ_is_expr_typ_def
-      (fun _ => True) (fun _ => True) (fun _ => True).
+      _ normᵗ_idem_def normᶜ_idem_def
+      normᶠ_idem_def normᵖ_idem_def.
 
-  Local Hint Constructors is_expr_typ : core.
-
-  Lemma uninit_sval_of_typ_is_expr_typ : forall t,
-      uninit_sval_of_typ_is_expr_typ_def t.
+  Ltac list_idem :=
+    intros ts Hts; f_equal;
+    apply map_ext_Forall in Hts;
+    rewrite map_map; auto; assumption.
+  
+  Ltac alist_idem :=
+    intros xts Hxts; f_equal;
+    pose proof Forall_map
+         (fun t => normᵗ (normᵗ t) = normᵗ t) snd xts
+      as H; unfold Basics.compose in H;
+    rewrite <- H in Hxts; clear H;
+    apply map_ext_Forall in Hxts;
+    repeat rewrite map_pat_combine;
+    repeat rewrite map_fst_combine;
+    repeat rewrite map_snd_combine;
+    repeat rewrite map_length; auto;
+    repeat rewrite map_id; rewrite map_map;
+    f_equal; auto; assumption.
+    
+  Lemma normᵗ_idem : forall t, normᵗ_idem_def t.
   Proof.
-    apply uninit_sval_of_typ_is_expr_typ_ind;
-      unfold uninit_sval_of_typ_is_expr_typ_def; cbn; auto.
-    - intros t n IH b v H.
-      destruct (uninit_sval_of_typ b t) as [v' |] eqn:Hv'; cbn in *;
-        unfold option_ret in H; inversion H; subst; clear H.
-      apply IH in Hv'. Fail apply is_array.
-  Abort.
+    apply normᵗ_idem_ind;
+      unfold normᵗ_idem_def,normᶜ_idem_def,
+      normᶠ_idem_def,normᵖ_idem_def; cbn in *;
+        try (intros; f_equal; eauto; assumption);
+        try list_idem; try alist_idem; eauto.
+    - intros X [t |] ms H; inversion H; subst; cbn; do 2 f_equal; auto.
+    - intros ds cs Hds Hcs.
+      apply map_ext_Forall in Hds, Hcs.
+      repeat rewrite map_map; f_equal; auto.
+    - intros Xs ws ps H.
+      apply map_ext_Forall in H.
+      repeat rewrite map_map; f_equal; auto.
+    - intros t ts Hts Ht.
+      apply map_ext_Forall in Hts;
+        rewrite map_map; f_equal; auto.
+    - intros Xs ws ps t Hps Ht.
+      apply map_ext_Forall in Hps;
+        rewrite map_map; f_equal; auto.
+    - intros Xs ps Hps;
+        apply map_ext_Forall in Hps;
+        rewrite map_map; f_equal; auto.
+    - intros Xs ps k t Hps Ht;
+        apply map_ext_Forall in Hps;
+        rewrite map_map; f_equal; auto.
+  Qed.
 End Lemmas.
